Squashed commit of the following:
commit 32f5885b5083c6052251a266b0ec4b6f0cd01bcc
Author: Jonas Kastberg Hinrichsen <jkas@itu.dk>
Date:   Tue Jun 11 11:54:32 2019 +0200

    Full bump

commit 3fdf913129ee6c1081e947de48e71ca6411f33da
Author: Robbert Krebbers <mail@robbertkrebbers.nl>
Date:   Tue Jun 11 11:31:22 2019 +0200

    More cleanup.

commit 46be8c0184d5a9e7de42022e389e23df99f73f6d
Author: Robbert Krebbers <mail@robbertkrebbers.nl>
Date:   Mon Jun 10 22:50:02 2019 +0200

    Some cleanup.

commit 2dc17e2cafc0b33e5ef0d2a6f6862b0938f68b18
Author: Jonas Kastberg Hinrichsen <jkas@itu.dk>
Date:   Mon Jun 10 16:33:46 2019 +0200

    WIP

commit 9427aa2ddd4fecb49b8e1c02eccc954fdb8af554
Author: Jonas Kastberg Hinrichsen <jkas@itu.dk>
Date:   Mon Jun 10 15:02:21 2019 +0200

    iRewrite Bug inspection

commit 40393f8800ab1a587f49f9ad479f5dc94b2bf2bc
Author: Jonas Kastberg Hinrichsen <jkas@itu.dk>
Date:   Mon Jun 10 14:56:08 2019 +0200

    Bumped Iris

commit 660218ca36e148b7270fd0044a2401fa553373d1
Author: Robbert Krebbers <mail@robbertkrebbers.nl>
Date:   Mon Jun 3 11:31:11 2019 +0200

    Add type.

commit 54214779390c19b1f9c8b293ac26f36efda95f4d
Author: Robbert Krebbers <mail@robbertkrebbers.nl>
Date:   Fri May 31 16:24:05 2019 +0200

    Coinductive version of stype.

commit b0fe9afb62c21df3b320d7ca13b92b3d60149c3b
Author: Robbert Krebbers <mail@robbertkrebbers.nl>
Date:   Fri May 31 13:19:13 2019 +0200

    Bump Iris.

theories/encodings/stype.v
@@ -20,28 +20,77 @@ Definition logrelΣ A :=
 Instance subG_chanΣ {A Σ} : subG (logrelΣ A) Σ → logrelG A Σ.
 Proof. intros [??%subG_auth_exclG]%subG_inv. constructor; apply _. Qed.
 
-Section stype_interp.
-  Context `{!heapG Σ} (N : namespace).
-  Context `{!logrelG val Σ}.
+Fixpoint st_eval `{!logrelG val Σ} (vs : list val) (st1 st2 : stype val (iProp Σ)) : iProp Σ :=
+  match vs with
+  | [] => st1 ≡ dual_stype st2
+  | v::vs => match st2 with
+             | TSR Receive P st2  => P v ∗ ▷ st_eval vs st1 (st2 v)
+             | _ => False
+             end
+  end%I.
+Arguments st_eval : simpl nomatch.
 
-  Record st_name := SessionType_name {
-    st_c_name : chan_name;
-    st_l_name : gname;
-    st_r_name : gname
-  }.
+Record st_name := STName {
+  st_c_name : chan_name;
+  st_l_name : gname;
+  st_r_name : gname
+}.
 
-  Definition to_stype_auth_excl (st : stype val (iProp Σ)) :=
-    to_auth_excl (Next (stype_map iProp_unfold st)).
+Definition to_stype_auth_excl `{!logrelG val Σ} (st : stype val (iProp Σ)) :=
+  to_auth_excl (Next (stype_map iProp_unfold st)).
 
-  Definition st_own (γ : st_name) (s : side)
-             (st : stype val (iProp Σ)) : iProp Σ :=
-    own (side_elim s st_l_name st_r_name γ)
-        (◯ to_stype_auth_excl st)%I.
+Definition st_own `{!logrelG val Σ} (γ : st_name) (s : side)
+    (st : stype val (iProp Σ)) : iProp Σ :=
+  own (side_elim s st_l_name st_r_name γ) (◯ to_stype_auth_excl st)%I.
 
-  Definition st_ctx (γ : st_name) (s : side)
-             (st : stype val (iProp Σ)) : iProp Σ :=
-    own (side_elim s st_l_name st_r_name γ)
-        (● to_stype_auth_excl st)%I.
+Definition st_ctx `{!logrelG val Σ} (γ : st_name) (s : side)
+    (st : stype val (iProp Σ)) : iProp Σ :=
+  own (side_elim s st_l_name st_r_name γ) (● to_stype_auth_excl st)%I.
+
+Definition inv_st `{!logrelG val Σ} (γ : st_name) (c : val) : iProp Σ :=
+  (∃ l r stl str,
+    chan_own (st_c_name γ) Left l ∗
+    chan_own (st_c_name γ) Right r ∗
+    st_ctx γ Left stl  ∗
+    st_ctx γ Right str ∗
+    ▷ ((⌜r = []⌝ ∗ st_eval l stl str) ∨
+       (⌜l = []⌝ ∗ st_eval r str stl)))%I.
+
+Definition interp_st `{!logrelG val Σ, !heapG Σ} (N : namespace) (γ : st_name)
+    (c : val) (s : side) (st : stype val (iProp Σ)) : iProp Σ :=
+  (st_own γ s st ∗ is_chan N (st_c_name γ) c ∗ inv N (inv_st γ c))%I.
+Instance: Params (@interp_st) 7.
+
+Notation "⟦ c @ s : st ⟧{ N , γ }" := (interp_st N γ c s st)
+  (at level 10, s at next level, st at next level, γ at next level,
+   format "⟦  c  @  s  :  st  ⟧{ N , γ }").
+
+Section stype.
+  Context `{!logrelG val Σ, !heapG Σ} (N : namespace).
+
+  Global Instance st_eval_ne : NonExpansive2 (st_eval vs).
+  Proof.
+    induction vs as [|v vs IH];
+      destruct 2 as [n|[] P1 P2 st1 st2|n [] P1 P2 st1 st2]=> //=.
+    - by repeat f_equiv.
+    - f_equiv. done. f_equiv. by constructor.
+    - f_equiv. done. f_equiv. by constructor.
+    - f_equiv. done. f_equiv. by constructor.
+    - f_equiv. done. f_equiv. by constructor.
+    - f_equiv. done. by f_contractive.
+    - f_equiv. done. f_contractive. apply IH. by apply dist_S. done.
+  Qed.
+  Global Instance st_eval_proper vs : Proper ((≡) ==> (≡) ==> (≡)) (st_eval vs).
+  Proof. apply (ne_proper_2 _). Qed.
+
+  Global Instance to_stype_auth_excl_ne : NonExpansive to_stype_auth_excl.
+  Proof. solve_proper. Qed.
+  Global Instance st_own_ne γ s : NonExpansive (st_own γ s).
+  Proof. solve_proper. Qed.
+  Global Instance interp_st_ne γ c s : NonExpansive (interp_st N γ c s).
+  Proof. solve_proper. Qed.
+  Global Instance interp_st_proper γ c s : Proper ((≡) ==> (≡)) (interp_st N γ c s).
+  Proof. apply (ne_proper _). Qed.
 
   Lemma st_excl_eq γ s st st' :
     st_ctx γ s st -∗ st_own γ s st' -∗ ▷ (st ≡ st').
@@ -58,8 +107,7 @@ Section stype_interp.
   Qed.
 
   Lemma st_excl_update γ s st st' st'' :
-    st_ctx γ s st -∗ st_own γ s st' ==∗
-    st_ctx γ s st'' ∗ st_own γ s st''.
+    st_ctx γ s st -∗ st_own γ s st' ==∗ st_ctx γ s st'' ∗ st_own γ s st''.
   Proof.
     iIntros "Hauth Hfrag".
     iDestruct (own_update_2 with "Hauth Hfrag") as "H".
@@ -67,130 +115,43 @@ Section stype_interp.
                               (to_stype_auth_excl st'')).
       eapply option_local_update.
       eapply exclusive_local_update. done. }
-    rewrite own_op.
-    done.
+    by rewrite own_op.
   Qed.
 
-  Fixpoint st_eval (vs : list val) (st1 st2 : stype val (iProp Σ)) : iProp Σ :=
-    match vs with
-    | [] => st1 ≡ dual_stype st2
-    | v::vs => match st2 with
-               | TSR Receive P st2  => P v ∗ st_eval vs st1 (st2 v)
-               | _ => False
-               end
-    end%I.
-  Global Arguments st_eval : simpl nomatch.
-
-  Lemma st_later_eq a P2 (st : stype val (iProp Σ)) st2 :
-    (▷ (st ≡ TSR a P2 st2) -∗
-         ◇ (∃ P1 st1, st ≡ TSR a P1 st1 ∗
-                       ▷ ((∀ v, P1 v ≡ P2 v)) ∗
-                       ▷ ((∀ v, st1 v ≡ st2 v))) : iProp Σ).
-  Proof.
-    destruct st.
-    - iIntros "Heq".
-      iDestruct (stype_equivI with "Heq") as ">Heq".
-      done.
-    - iIntros "Heq".
-      iDestruct (stype_equivI with "Heq") as "Heq".
-      iDestruct ("Heq") as "[>Haeq [HPeq Hsteq]]".
-      iDestruct "Haeq" as %Haeq.
-      subst.
-      iExists P, st.
-      iSplit=> //.
-      by iSplitL "HPeq".
-  Qed.
-
-  Global Instance st_eval_ne : NonExpansive2 (st_eval vs).
-  Proof.
-    intros vs n. induction vs as [|v vs IH]; [solve_proper|].
-    destruct 2 as [|[] ????? Hst]=> //=. f_equiv. solve_proper.
-    by apply IH, Hst.
-  Qed.
-
-  Lemma st_eval_send (P : val -> iProp Σ) st l str v :
-    P v -∗ st_eval l (TSR Send P st) str -∗ st_eval (l ++ [v]) (st v) str.
+  Lemma st_eval_send (P : val →iProp Σ) st vs v str :
+    P v -∗ st_eval vs (<!> @ P, st) str -∗ st_eval (vs ++ [v]) (st v) str.
   Proof.
     iIntros "HP".
     iRevert (str).
-    iInduction l as [|l] "IH"; iIntros (str) "Heval".
-    - simpl.
-      iDestruct (dual_stype_flip with "Heval") as "Heval".
-      iRewrite -"Heval". simpl.
+    iInduction vs as [|v' vs] "IH"; iIntros (str) "Heval".
+    - iDestruct (dual_stype_flip with "Heval") as "Heval".
+      iRewrite -"Heval"; simpl.
       rewrite dual_stype_involutive.
       by iFrame.
-    - simpl.
-      destruct str; auto.
-      destruct a; auto.
-      iDestruct "Heval" as "[HP0 Heval]".
-      iFrame.
+    - destruct str as [|[] P' str]=> //=.
+      iDestruct "Heval" as "[$ Heval]".
       by iApply ("IH" with "HP").
   Qed.
 
   Lemma st_eval_recv (P : val → iProp Σ) st1 l st2 v :
-     st_eval (v :: l) st1 (TSR Receive P st2) -∗ st_eval l st1 (st2 v) ∗ P v.
+     st_eval (v :: l) st1 (<?> @ P, st2) -∗ ▷ st_eval l st1 (st2 v) ∗ P v.
   Proof. iDestruct 1 as "[HP Heval]". iFrame. Qed.
-
-  Definition inv_st (γ : st_name) (c : val) : iProp Σ :=
-    (∃ l r stl str,
-      chan_own (st_c_name γ) Left l ∗
-      chan_own (st_c_name γ) Right r ∗
-      st_ctx γ Left stl  ∗
-      st_ctx γ Right str ∗
-      ((⌜r = []⌝ ∗ st_eval l stl str) ∨
-       (⌜l = []⌝ ∗ st_eval r str stl)))%I.
-
-  Definition is_st (γ : st_name) (st : stype val (iProp Σ))
-      (c : val) : iProp Σ :=
-    (is_chan N (st_c_name γ) c ∗ inv N (inv_st γ c))%I.
-
-  Definition interp_st (γ : st_name) (st : stype val (iProp Σ))
-      (c : val) (s : side) : iProp Σ :=
-    (st_own γ s st ∗ is_st γ st c)%I.
-
-  Global Instance interp_st_proper γ :
-    Proper ((≡) ==> (=) ==> (=) ==> (≡)) (interp_st γ).
-  Proof.
-    intros st1 st2 Heq v1 v2 <- s1 s2 <-.
-    iSplit;
-    iIntros "[Hown Hctx]";
-    iFrame;
-    unfold st_own;
-    iApply (own_mono with "Hown");
-    apply (auth_frag_mono);
-    apply Some_included;
-    left;
-    f_equiv;
-    f_equiv;
-    apply stype_map_equiv=> //.
-  Qed.
-End stype_interp.
-
-Notation "⟦ c @ s : st ⟧{ N , γ }" := (interp_st N γ st c s)
-  (at level 10, s at next level, st at next level, γ at next level,
-   format "⟦  c  @  s  :  st  ⟧{ N , γ }").
-
-Section stype_specs.
-  Context `{!heapG Σ} (N : namespace).
-  Context `{!logrelG val Σ}.
 
   Lemma new_chan_vs st E c cγ :
     is_chan N cγ c ∗
     chan_own cγ Left [] ∗
-    chan_own cγ Right []
-    ={E}=∗
-      ∃ lγ rγ,
-        let γ := SessionType_name cγ lγ rγ in
-        ⟦ c @ Left : st ⟧{N,γ} ∗ ⟦ c @ Right : dual_stype st ⟧{N,γ}.
+    chan_own cγ Right [] ={E}=∗ ∃ lγ rγ,
+      let γ := STName cγ lγ rγ in
+      ⟦ c @ Left : st ⟧{N,γ} ∗ ⟦ c @ Right : dual_stype st ⟧{N,γ}.
   Proof.
     iIntros "[#Hcctx [Hcol Hcor]]".
     iMod (own_alloc (● (to_stype_auth_excl st) ⋅
-                     ◯ (to_stype_auth_excl st)))
-      as (lγ) "[Hlsta Hlstf]"; first done.
+                     ◯ (to_stype_auth_excl st))) as (lγ) "[Hlsta Hlstf]".
+    { by apply auth_both_valid_2. }
     iMod (own_alloc (● (to_stype_auth_excl (dual_stype st)) ⋅
-                     ◯ (to_stype_auth_excl (dual_stype st))))
-      as (rγ) "[Hrsta Hrstf]"; first done.
-    pose (SessionType_name cγ lγ rγ) as stγ.
+                     ◯ (to_stype_auth_excl (dual_stype st)))) as (rγ) "[Hrsta Hrstf]".
+    { by apply auth_both_valid_2. }
+    pose (STName cγ lγ rγ) as stγ.
     iMod (inv_alloc N _ (inv_st stγ c) with "[-Hlstf Hrstf Hcctx]") as "#Hinv".
     { iNext. rewrite /inv_st. eauto 10 with iFrame. }
     iModIntro.
@@ -202,8 +163,7 @@ Section stype_specs.
     IsDualStype st1 st2 →
     {{{ True }}}
       new_chan #()
-    {{{ c γ, RET c;  ⟦ c @ Left : st1 ⟧{N,γ} ∗
-                     ⟦ c @ Right : st2 ⟧{N,γ} }}}.
+    {{{ c γ, RET c; ⟦ c @ Left : st1 ⟧{N,γ} ∗ ⟦ c @ Right : st2 ⟧{N,γ} }}}.
   Proof.
     rewrite /IsDualStype.
     iIntros (Hst Φ _) "HΦ".
@@ -221,49 +181,41 @@ Section stype_specs.
 
   Lemma send_vs c γ s (P : val → iProp Σ) st E :
     ↑N ⊆ E →
-    ⟦ c @ s : TSR Send P st ⟧{N,γ} ={E,E∖↑N}=∗
-      ∃ vs, chan_own (st_c_name γ) s vs ∗
-      ▷ (∀ v, P v -∗
-              chan_own (st_c_name γ) s (vs ++ [v])
-              ={E∖ ↑N,E}=∗ ⟦ c @ s : st v ⟧{N,γ}).
+    ⟦ c @ s : TSR Send P st ⟧{N,γ} ={E,E∖↑N}=∗ ∃ vs,
+      chan_own (st_c_name γ) s vs ∗
+      ▷ ∀ v, P v -∗
+             chan_own (st_c_name γ) s (vs ++ [v]) ={E∖↑N,E}=∗
+             ⟦ c @ s : st v ⟧{N,γ}.
   Proof.
     iIntros (Hin) "[Hstf #[Hcctx Hinv]]".
-    iMod (inv_open with "Hinv") as "Hinv'"=> //.
-    iDestruct "Hinv'" as "[Hinv' Hinvstep]".
-    iDestruct "Hinv'" as
-        (l r stl str) "(>Hclf & >Hcrf & Hstla & Hstra & Hinv')".
+    iInv N as (l r stl str) "(>Hclf & >Hcrf & Hstla & Hstra & Hinv')" "Hclose".
     iModIntro.
     destruct s.
     - iExists _.
       iIntros "{$Hclf} !>" (v) "HP Hclf".
       iRename "Hstf" into "Hstlf".
       iDestruct (st_excl_eq with "Hstla Hstlf") as "#Heq".
-      iMod (st_excl_update _ _ _ _ (st v) with "Hstla Hstlf")
-        as "[Hstla Hstlf]".
-      iMod ("Hinvstep" with "[-Hstlf]") as "_".
-      {
-        iNext.
+      iMod (st_excl_update _ _ _ _ (st v) with "Hstla Hstlf") as "[Hstla Hstlf]".
+      iMod ("Hclose" with "[-Hstlf]") as "_".
+      { iNext.
         iExists _,_,_,_. iFrame.
         iLeft.
         iDestruct "Hinv'" as "[[-> Heval]|[-> Heval]]".
         - iSplit=> //.
           iApply (st_eval_send with "HP").
-          by iRewrite -"Heq".
-        - iRewrite "Heq" in "Heval". destruct r as [|vr r]=> //.
-          iSplit; first done. simpl.
-          iRewrite "Heval". simpl. iFrame "HP". by rewrite involutive.
-      }
-      iModIntro. iFrame. rewrite /is_st. auto.
+          by iRewrite "Heq" in "Heval".
+        - iRewrite "Heq" in "Heval". destruct r as [|vr r]=> //=.
+          iSplit; first done.
+          iRewrite "Heval". simpl. iFrame "HP". by rewrite involutive. }
+      iModIntro. iFrame. auto.
     - iExists _.
       iIntros "{$Hcrf} !>" (v) "HP Hcrf".
       iRename "Hstf" into "Hstrf".
       iDestruct (st_excl_eq with "Hstra Hstrf") as "#Heq".
-      iMod (st_excl_update _ _ _ _ (st v) with "Hstra Hstrf")
-        as "[Hstra Hstrf]".
-      iMod ("Hinvstep" with "[-Hstrf]") as "_".
-      {
-        iNext.
-        iExists _,_,_,_. iFrame.
+      iMod (st_excl_update _ _ _ _ (st v) with "Hstra Hstrf") as "[Hstra Hstrf]".
+      iMod ("Hclose" with "[-Hstrf]") as "_".
+      { iNext.
+        iExists _, _, _, _. iFrame.
         iRight.
         iDestruct "Hinv'" as "[[-> Heval]|[-> Heval]]".
         - iRewrite "Heq" in "Heval". destruct l as [|vl l]=> //.
@@ -271,9 +223,8 @@ Section stype_specs.
           iRewrite "Heval". simpl. iFrame "HP". by rewrite involutive.
         - iSplit=> //.
           iApply (st_eval_send with "HP").
-            by iRewrite -"Heq".
-      }
-      iModIntro. iFrame. rewrite /is_st. auto.
+          by iRewrite "Heq" in "Heval". }
+      iModIntro. iFrame. auto.
   Qed.
 
   Lemma send_st_spec st γ c s (P : val → iProp Σ) v :
@@ -292,75 +243,60 @@ Section stype_specs.
 
   Lemma try_recv_vs c γ s (P : val → iProp Σ) st E :
     ↑N ⊆ E →
-    ⟦ c @ s : TSR Receive P st ⟧{N,γ}
-    ={E,E∖↑N}=∗
-      ∃ vs, chan_own (st_c_name γ) (dual_side s) vs ∗
-      (▷ ((⌜vs = []⌝ -∗ chan_own (st_c_name γ) (dual_side s) vs ={E∖↑N,E}=∗
+    ⟦ c @ s : TSR Receive P st ⟧{N,γ} ={E,E∖↑N}=∗ ∃ vs,
+      chan_own (st_c_name γ) (dual_side s) vs ∗
+      ▷ ((⌜vs = []⌝ -∗
+           chan_own (st_c_name γ) (dual_side s) vs ={E∖↑N,E}=∗
            ⟦ c @ s : TSR Receive P st ⟧{N,γ}) ∧
-          (∀ v vs', ⌜vs = v :: vs'⌝ -∗
-               chan_own (st_c_name γ) (dual_side s) vs' -∗ |={E∖↑N,E}=>
-               ⟦ c @ s : (st v) ⟧{N,γ} ∗ ▷  P v))).
+         (∀ v vs',
+           ⌜vs = v :: vs'⌝ -∗
+           chan_own (st_c_name γ) (dual_side s) vs' ={E∖↑N,E}=∗
+           ⟦ c @ s : (st v) ⟧{N,γ} ∗ ▷ P v)).
   Proof.
     iIntros (Hin) "[Hstf #[Hcctx Hinv]]".
-    iMod (inv_open with "Hinv") as "Hinv'"=> //.
-    iDestruct "Hinv'" as "[Hinv' Hinvstep]".
-    iDestruct "Hinv'" as
-        (l r stl str) "(>Hclf & >Hcrf & Hstla & Hstra & Hinv')".
+    iInv N as (l r stl str) "(>Hclf & >Hcrf & Hstla & Hstra & Hinv')" "Hclose".
     iExists (side_elim s r l). iModIntro.
-    destruct s.
-    - simpl. iIntros "{$Hcrf} !>".
+    destruct s; simpl.
+    - iIntros "{$Hcrf} !>".
       iRename "Hstf" into "Hstlf".
       iDestruct (st_excl_eq with "Hstla Hstlf") as "#Heq".
-      iSplit=> //.
-      + iIntros "Hvs Hown".
-        iMod ("Hinvstep" with "[-Hstlf]") as "_".
-        { iNext. iExists l,r,_,_. iFrame. }
+      iSplit.
+      + iIntros (->) "Hown".
+        iMod ("Hclose" with "[-Hstlf]") as "_".
+        { iNext. iExists l, [], _, _. iFrame. }
         iModIntro. iFrame "Hcctx ∗ Hinv".
-      + iIntros (v vs Hvs) "Hown".
-        iDestruct "Hinv'" as "[[-> Heval]|[-> Heval]]"; first inversion Hvs.
-        iMod (st_excl_update _ _ _ _ (st v) with "Hstla Hstlf")
-          as "[Hstla Hstlf]".
-        subst.
-        iDestruct (st_later_eq with "Heq") as ">Hleq".
-        iDestruct "Hleq" as (P1 st1) "[Hsteq [HPeq Hsteq']]".
-        iSpecialize ("HPeq" $!v).
-        iSpecialize ("Hsteq'" $!v).
+      + iIntros (v vs ->) "Hown".
+        iDestruct "Hinv'" as "[[>% _]|[> -> Heval]]"; first done.
+        iMod (st_excl_update _ _ _ _ (st v) with "Hstla Hstlf") as "[Hstla Hstlf]".
+        iDestruct (stype_later_equiv with "Heq") as ">Hleq".
+        iDestruct "Hleq" as (P1 st1) "(Hsteq & HPeq & Hsteq')".
         iRewrite "Hsteq" in "Heval".
-        subst.
         iDestruct (st_eval_recv with "Heval") as "[Heval HP]".
-        iMod ("Hinvstep" with "[-Hstlf HP]") as "H".
-        { iExists _,_,_,_. iFrame. iRight=> //.
-          iNext. iSplit=> //. by iRewrite -"Hsteq'". }
-        iModIntro.
-        iSplitR "HP".
-        * iFrame "Hstlf Hcctx Hinv".
-        * iNext. by iRewrite -"HPeq".
-    - simpl. iIntros "{$Hclf} !>".
+        iMod ("Hclose" with "[-Hstlf HP]") as "H".
+        { iExists _, _,_ ,_. iFrame. iRight.
+          iNext. iSplit=> //. iNext. by iRewrite -("Hsteq'" $! v). }
+        iModIntro. iFrame "Hstlf Hcctx Hinv".
+        iNext. by iRewrite -("HPeq" $! v).
+    - iIntros "{$Hclf} !>".
       iRename "Hstf" into "Hstrf".
       iDestruct (st_excl_eq with "Hstra Hstrf") as "#Heq".
       iSplit=> //.
-      + iIntros "Hvs Hown".
-        iMod ("Hinvstep" with "[-Hstrf]") as "_".
-        { iNext. iExists l,r,_,_. iFrame. }
+      + iIntros (->) "Hown".
+        iMod ("Hclose" with "[-Hstrf]") as "_".
+        { iNext. iExists [], r, _, _. iFrame. }
         iModIntro. iFrame "Hcctx ∗ Hinv".
-      + iIntros (v vs' Hvs) "Hown".
-        iDestruct "Hinv'" as "[[-> Heval]|[-> Heval]]"; last inversion Hvs.
-        iMod (st_excl_update _ _ _ _ (st v) with "Hstra Hstrf")
-          as "[Hstra Hstrf]".
-        subst.
-        iDestruct (st_later_eq with "Heq") as ">Hleq".
-        iDestruct "Hleq" as (P1 st1) "[Hsteq [HPeq Hsteq']]".
-        iSpecialize ("HPeq" $!v).
-        iSpecialize ("Hsteq'" $!v).
+      + iIntros (v vs' ->) "Hown".
+        iDestruct "Hinv'" as "[[>-> Heval]|[>% Heval]]"; last done.
+        iMod (st_excl_update _ _ _ _ (st v) with "Hstra Hstrf") as "[Hstra Hstrf]".
+        iDestruct (stype_later_equiv with "Heq") as ">Hleq".
+        iDestruct "Hleq" as (P1 st1) "(Hsteq & HPeq & Hsteq')".
         iRewrite "Hsteq" in "Heval".
         iDestruct (st_eval_recv with "Heval") as "[Heval HP]".
-        iMod ("Hinvstep" with "[-Hstrf HP]") as "_".
-        { iExists _,_,_,_. iFrame. iLeft=> //.
-            iNext. iSplit=> //. by iRewrite -"Hsteq'". }
-        iModIntro.
-        iSplitR "HP".
-        * iFrame "Hstrf Hcctx Hinv".
-        * iNext. by iRewrite -"HPeq".
+        iMod ("Hclose" with "[-Hstrf HP]") as "_".
+        { iExists _, _, _, _. iFrame. iLeft.
+          iNext. iSplit=> //. iNext. by iRewrite -("Hsteq'" $! v). }
+        iModIntro. iFrame "Hstrf Hcctx Hinv".
+        iNext. by iRewrite -("HPeq" $! v).
   Qed.
 
   Lemma try_recv_st_spec st γ c s (P : val → iProp Σ) :
@@ -378,39 +314,29 @@ Section stype_specs.
     iSplit.
     - iIntros (Hvs) "Hown".
       iDestruct "H" as "[H _]".
-      iSpecialize ("H" $!Hvs).
-      iMod ("H" with "Hown") as "H".
+      iMod ("H" $!Hvs with "Hown") as "H".
       iModIntro.
       iApply "HΦ"=> //.
       eauto with iFrame.
     - iIntros (v vs' Hvs) "Hown".
       iDestruct "H" as "[_ H]".
-      iSpecialize ("H" $!v vs' Hvs).
-      iMod ("H" with "Hown") as "H".
+      iMod ("H" $!v vs' Hvs with "Hown") as "H".
       iModIntro.
-      iApply "HΦ"=> //.
-      eauto with iFrame.
+      iApply "HΦ"; eauto with iFrame.
   Qed.
 
   Lemma recv_st_spec st γ c s (P : val → iProp Σ) :
     {{{ ⟦ c @ s : <?> @ P ,  st ⟧{N,γ} }}}
       recv c #s
-    {{{ v, RET v; ⟦ c @ s : st v ⟧{N,γ} ∗ P v}}}.
+    {{{ v, RET v; ⟦ c @ s : st v ⟧{N,γ} ∗ P v }}}.
   Proof.
     iIntros (Φ) "Hrecv HΦ".
     iLöb as "IH". wp_rec.
     wp_apply (try_recv_st_spec with "Hrecv").
     iIntros (v) "H".
-    iDestruct "H" as "[H | H]".
-    - iDestruct "H" as "[Hv H]".
-      iDestruct "Hv" as %->.
-      wp_pures.
-      iApply ("IH" with "[H]")=> //.
-    - iDestruct "H" as (w) "[Hv [H HP]]".
-      iDestruct "Hv" as %->.
-      wp_pures.
-      iApply "HΦ".
-      iFrame.
+    iDestruct "H" as "[[-> H]| H]".
+    - wp_pures. by iApply ("IH" with "[H]").
+    - iDestruct "H" as (w ->) "[H HP]".
+      wp_pures. iApply "HΦ". iFrame.
   Qed.
-
-End stype_specs.
+End stype.
