theories/typing/stype.v
@@ -14,7 +14,7 @@ Definition dual_action (a : action) : action :=
 Instance dual_action_involutive : Involutive (=) dual_action.
 Proof. by intros []. Qed.
 
-Inductive stype (V A : Type) :=
+CoInductive stype (V A : Type) :=
   | TEnd
   | TSR (a : action) (P : V → A) (st : V → stype V A).
 Arguments TEnd {_ _}.
@@ -23,7 +23,7 @@ Instance: Params (@TSR) 3.
 
 Instance stype_inhabited V A : Inhabited (stype V A) := populate TEnd.
 
-Fixpoint dual_stype {V A} (st : stype V A) :=
+CoFixpoint dual_stype {V A} (st : stype V A) : stype V A :=
   match st with
   | TEnd => TEnd
   | TSR a P st => TSR (dual_action a) P (λ v, dual_stype (st v))
@@ -52,7 +52,7 @@ Section stype_ofe.
   Context {V : Type}.
   Context {A : ofeT}.
 
-  Inductive stype_equiv : Equiv (stype V A) :=
+  CoInductive stype_equiv : Equiv (stype V A) :=
     | TEnd_equiv : TEnd ≡ TEnd
     | TSR_equiv a P1 P2 st1 st2 :
        pointwise_relation V (≡) P1 P2 →
@@ -60,79 +60,119 @@ Section stype_ofe.
        TSR a P1 st1 ≡ TSR a P2 st2.
   Existing Instance stype_equiv.
 
-  Inductive stype_dist' (n : nat) : relation (stype V A) :=
-    | TEnd_dist : stype_dist' n TEnd TEnd
-    | TSR_dist a P1 P2 st1 st2 :
-       pointwise_relation V (dist n) P1 P2 →
-       pointwise_relation V (stype_dist' n) st1 st2 →
-       stype_dist' n (TSR a P1 st1) (TSR a P2 st2).
-  Instance stype_dist : Dist (stype V A) := stype_dist'.
+  CoInductive stype_dist : Dist (stype V A) :=
+    | TEnd_dist n : TEnd ≡{n}≡ TEnd
+    | TSR_dist_0 a P1 P2 st1 st2 :
+       pointwise_relation V (dist 0) P1 P2 →
+       TSR a P1 st1 ≡{0}≡ TSR a P2 st2
+    | TSR_dist_S n a P1 P2 st1 st2 :
+       pointwise_relation V (dist (S n)) P1 P2 →
+       pointwise_relation V (dist n) st1 st2 →
+       TSR a P1 st1 ≡{S n}≡ TSR a P2 st2.
+  Existing Instance stype_dist.
+
+  Lemma TSR_dist n a P1 P2 st1 st2 :
+    pointwise_relation V (dist n) P1 P2 →
+    pointwise_relation V (dist_later n) st1 st2 →
+    TSR a P1 st1 ≡{n}≡ TSR a P2 st2.
+  Proof. destruct n; by constructor. Defined.
 
   Definition stype_ofe_mixin : OfeMixin (stype V A).
   Proof.
     split.
-    - intros st1 st2. rewrite /dist /stype_dist. split.
-      + intros Hst n.
-        induction Hst as [|a P1 P2 st1 st2 HP Hst IH]; constructor; intros v.
-        * apply equiv_dist, HP.
-        * apply IH.
-      + revert st2. induction st1 as [|a P1 st1 IH]; intros [|a' P2 st2] Hst.
-        * constructor.
-        * feed inversion (Hst O).
-        * feed inversion (Hst O).
-        * feed inversion (Hst O); subst.
-          constructor; intros v.
-          ** apply equiv_dist=> n. feed inversion (Hst n); subst; auto.
-          ** apply IH=> n. feed inversion (Hst n); subst; auto.
-    - rewrite /dist /stype_dist. split.
-      + intros st. induction st; constructor; repeat intro; auto.
-      + intros st1 st2. induction 1; constructor; repeat intro; auto.
-        symmetry; auto.
-      + intros st1 st2 st3 H1 H2.
-        revert H2. revert st3.
-        induction H1 as [| a P1 P2 st1 st2 HP Hst12 IH]=> //.
-        inversion 1. subst. constructor.
-        ** by transitivity P2.
-        ** intros v. by apply IH.
-    - intros n st1 st2. induction 1; constructor.
-      + intros v. apply dist_S. apply H.
-      + intros v. apply H1.
+    - intros st1 st2. split.
+      + revert st1 st2. cofix IH; destruct 1 as [|a P1 P2 st1' st2' HP]=> n.
+        { constructor. }
+        destruct n as [|n].
+        * constructor=> v. apply equiv_dist, HP.
+        * constructor=> v. apply equiv_dist, HP. by apply IH.
+      + revert st1 st2. cofix IH=> -[|a1 P1 st1] -[|a2 P2 st2] Hst;
+          feed inversion (Hst O); subst; constructor=> v.
+        * apply equiv_dist=> n. feed inversion (Hst n); auto.
+        * apply IH=> n. feed inversion (Hst (S n)); auto.
+    - intros n. split.
+      + revert n. cofix IH=> -[|n] [|a P st]; constructor=> v; auto.
+      + revert n. cofix IH; destruct 1; constructor=> v; symmetry; auto.
+      + revert n. cofix IH; destruct 1; inversion 1; constructor=> v; etrans; eauto.
+    - cofix IH=> -[|n]; inversion 1; constructor=> v; try apply dist_S; auto.
   Qed.
   Canonical Structure stypeC : ofeT := OfeT (stype V A) stype_ofe_mixin.
 
+  Definition stype_head (d : V -c> A) (st : stype V A) : V -c> A :=
+    match st with TEnd => d | TSR a P st => P end.
+  Definition stype_tail (v : V) (st : stypeC) : later stypeC :=
+    match st with TEnd => Next TEnd | TSR a P st => Next (st v) end.
+  Global Instance stype_head_ne d : NonExpansive (stype_head d).
+  Proof. by destruct 1. Qed.
+  Global Instance stype_tail_ne v : NonExpansive (stype_tail v).
+  Proof. destruct 1; naive_solver. Qed.
+
+  Definition stype_force (st : stype V A) : stype V A :=
+    match st with
+    | TEnd => TEnd
+    | TSR a P st => TSR a P st
+    end.
+  Lemma stype_force_eq st : stype_force st = st.
+  Proof. by destruct st. Defined.
+
+  CoFixpoint stype_compl_go `{!Cofe A} (c : chain stypeC) : stypeC :=
+    match c O with
+    | TEnd => TEnd
+    | TSR a P st => TSR a
+       (compl (chain_map (stype_head P) c) : V → A)
+       (λ v, stype_compl_go (later_chain (chain_map (stype_tail v) c)))
+    end.
+
+  Global Program Instance stype_cofe `{!Cofe A} : Cofe stypeC :=
+    {| compl c := stype_compl_go c |}.
+  Next Obligation.
+    intros ? n c; rewrite /compl. revert c n. cofix IH=> c n.
+    rewrite -(stype_force_eq (stype_compl_go c)) /=.
+    destruct (c O) as [|a P st'] eqn:Hc0.
+    - assert (c n ≡{0}≡ TEnd) as Hcn.
+      { rewrite -Hc0 -(chain_cauchy c 0 n) //. lia. }
+      by inversion Hcn.
+    - assert (c n ≡{0}≡ TSR a P st') as Hcn.
+      { rewrite -Hc0 -(chain_cauchy c 0 n) //. lia. }
+      inversion Hcn as [|? P' ? st'' ? HP|]; subst.
+      destruct n as [|n]; constructor.
+      + intros v. by rewrite (conv_compl 0 (chain_map (stype_head P) c) v) /= -H.
+      + intros v. by rewrite (conv_compl _ (chain_map (stype_head P) c) v) /= -H.
+      + intros v. assert (st'' v = later_car (stype_tail v (c (S n)))) as ->.
+        { by rewrite -H /=. }
+        apply IH.
+  Qed.
+
+  Global Instance TSR_stype_contractive a n :
+    Proper (pointwise_relation _ (dist n) ==>
+            pointwise_relation _ (dist_later n) ==> dist n) (TSR a).
+  Proof. destruct n; by constructor. Qed.
   Global Instance TSR_stype_ne a n :
     Proper (pointwise_relation _ (dist n) ==>
             pointwise_relation _ (dist n) ==> dist n) (TSR a).
   Proof.
-    intros P1 P2 HP st1 st2 Hst.
-    constructor.
-    - apply HP.
-    - intros v. apply Hst.
+    intros P1 P2 HP st1 st2 Hst. apply TSR_stype_contractive=> //.
+    destruct n as [|n]=> // v /=. by apply dist_S.
   Qed.
   Global Instance TSR_stype_proper a :
     Proper (pointwise_relation _ (≡) ==>
             pointwise_relation _ (≡) ==> (≡)) (TSR a).
-  Proof.
-    intros P1 P2 HP st1 st2 Hst. apply equiv_dist=> n.
-    by f_equiv; intros v; apply equiv_dist.
-  Qed.
+  Proof. by constructor. Qed.
 
   Global Instance dual_stype_ne : NonExpansive dual_stype.
   Proof.
-    intros n. induction 1 as [| a P1 P2 st1 st2 HP Hst IH].
-    - constructor.
-    - constructor. apply HP. intros v. apply IH.
+    cofix IH=> n st1 st2 Hst.
+    rewrite -(stype_force_eq (dual_stype st1)) -(stype_force_eq (dual_stype st2)).
+    destruct Hst; constructor=> v; auto; by apply IH.
   Qed.
   Global Instance dual_stype_proper : Proper ((≡) ==> (≡)) dual_stype.
   Proof. apply (ne_proper _). Qed.
 
   Global Instance dual_stype_involutive : Involutive (≡) dual_stype.
   Proof.
-    intros st.
-    induction st.
-    - constructor.
-    - rewrite /= (involutive (f:=dual_action)).
-      constructor. reflexivity. intros v. apply H.
+    cofix IH=> st. rewrite -(stype_force_eq (dual_stype (dual_stype _))).
+    destruct st as [|a P st]; first done.
+    rewrite /= involutive. constructor=> v; auto.
   Qed.
 
   Lemma stype_equivI {M} st1 st2 :
@@ -140,13 +180,25 @@ Section stype_ofe.
         match st1, st2 with
         | TEnd, TEnd => True
         | TSR a1 P1 st1, TSR a2 P2 st2 =>
-          ⌜ a1 = a2 ⌝ ∧ (∀ v, P1 v ≡ P2 v) ∧ (∀ v, st1 v ≡ st2 v)
+          ⌜ a1 = a2 ⌝ ∧ (∀ v, P1 v ≡ P2 v) ∧ ▷ (∀ v, st1 v ≡ st2 v)
         | _, _ => False
         end.
   Proof.
     uPred.unseal; constructor=> n x ?. split; first by destruct 1.
     destruct st1, st2=> //=; [constructor|].
-    by intros [[= ->] [??]]; constructor.
+    by intros [[= ->] [??]]; destruct n; constructor.
+  Qed.
+
+  Lemma stype_later_equiv M st a P2 st2 :
+    ▷ (st ≡ TSR a P2 st2) -∗
+    ◇ (∃ P1 st1, st ≡ TSR a P1 st1 ∗
+                 ▷ (∀ v, P1 v ≡ P2 v) ∗
+                 ▷ ▷ (∀ v, st1 v ≡ st2 v) : uPred M).
+  Proof.
+    iIntros "Heq". destruct st as [|a' P1 st1].
+    - iDestruct (stype_equivI with "Heq") as ">[]".
+    - iDestruct (stype_equivI with "Heq") as "(>-> & HPeq & Hsteq)".
+      iExists P1, st1. auto.
   Qed.
 
   Lemma dual_stype_flip {M} st1 st2 :
@@ -156,11 +208,11 @@ Section stype_ofe.
     - iIntros "Heq". iRewrite -"Heq". by rewrite dual_stype_involutive.
     - iIntros "Heq". iRewrite "Heq". by rewrite dual_stype_involutive.
   Qed.
-
 End stype_ofe.
+
 Arguments stypeC : clear implicits.
 
-Fixpoint stype_map {V A B} (f : A → B) (st : stype V A) : stype V B :=
+CoFixpoint stype_map {V A B} (f : A → B) (st : stype V A) : stype V B :=
   match st with
   | TEnd => TEnd
   | TSR a P st => TSR a (λ v, f (P v)) (λ v, stype_map f (st v))
@@ -168,42 +220,36 @@ Fixpoint stype_map {V A B} (f : A → B) (st : stype V A) : stype V B :=
 Lemma stype_map_ext_ne {V A} {B : ofeT} (f g : A → B) (st : stype V A) n :
   (∀ x, f x ≡{n}≡ g x) → stype_map f st ≡{n}≡ stype_map g st.
 Proof.
-  intros Hf. induction st as [| a P st IH]; constructor.
-  - intros v. apply Hf.
-  - intros v. apply IH.
+  revert n st. cofix IH=> n st Hf.
+  rewrite -(stype_force_eq (stype_map f st)) -(stype_force_eq (stype_map g st)).
+  destruct st as [|a P st], n as [|n]; constructor=> v //. apply IH; auto using dist_S.
 Qed.
 Lemma stype_map_ext {V A} {B : ofeT} (f g : A → B) (st : stype V A) :
   (∀ x, f x ≡ g x) → stype_map f st ≡ stype_map g st.
 Proof.
-  intros Hf. apply equiv_dist.
-  intros n. apply stype_map_ext_ne.
-  intros x. apply equiv_dist.
-  apply Hf.
+  intros Hf. apply equiv_dist=> n. apply stype_map_ext_ne=> v.
+  apply equiv_dist, Hf.
 Qed.
 Instance stype_map_ne {V : Type} {A B : ofeT} (f : A → B) n :
-  Proper (dist n ==> dist n) f →
+  (∀ n, Proper (dist n ==> dist n) f) →
   Proper (dist n ==> dist n) (@stype_map V _ _ f).
 Proof.
-  intros Hf st1 st2. induction 1 as [| a P1 P2 st1 st2 HP Hst IH]; constructor.
-  - intros v. f_equiv. apply HP.
-  - intros v. apply IH.
+  intros Hf. revert n. cofix IH=> n st1 st2 Hst.
+  rewrite -(stype_force_eq (stype_map _ st1)) -(stype_force_eq (stype_map _ st2)).
+  destruct Hst; constructor=> v; apply Hf || apply IH; auto.
 Qed.
-Lemma stype_map_equiv {A B : ofeT} (f g : A -n> B) (st st' : stype val A) :
-  (∀ x, f x ≡ g x) → st ≡ st' → stype_map f st ≡ stype_map g st'.
-Proof. intros Feq. induction 1=>//. constructor=>//. by repeat f_equiv. Qed.
 Lemma stype_fmap_id {V : Type} {A : ofeT} (st : stype V A) :
   stype_map id st ≡ st.
 Proof.
-  induction st as [| a P st IH]; constructor.
-  - intros v. reflexivity.
-  - intros v. apply IH.
+  revert st. cofix IH=> st. rewrite -(stype_force_eq (stype_map _ _)).
+  destruct st; constructor=> v; auto.
 Qed.
 Lemma stype_fmap_compose {V : Type} {A B C : ofeT} (f : A → B) (g : B → C) st :
   stype_map (g ∘ f) st ≡ stype_map g (@stype_map V _ _ f st).
 Proof.
-  induction st as [| a P st IH]; constructor.
-  - intros v. reflexivity.
-  - intros v. apply IH.
+  revert st. cofix IH=> st.
+  rewrite -(stype_force_eq (stype_map _ _)) -(stype_force_eq (stype_map g _)).
+  destruct st; constructor=> v; auto.
 Qed.
 
 Definition stypeC_map {V A B} (f : A -n> B) : stypeC V A -n> stypeC V B :=
@@ -212,25 +258,29 @@ Instance stypeC_map_ne {V} A B : NonExpansive (@stypeC_map V A B).
 Proof. intros n f g ? st. by apply stype_map_ext_ne. Qed.
 
 Program Definition stypeCF {V} (F : cFunctor) : cFunctor := {|
-  cFunctor_car A B := stypeC V (cFunctor_car F A B);
-  cFunctor_map A1 A2 B1 B2 fg := stypeC_map (cFunctor_map F fg)
+  cFunctor_car A _ B _ := stypeC V (cFunctor_car F A _ B _);
+  cFunctor_map A1 _ A2 _ B1 _ B2 _ fg := stypeC_map (cFunctor_map F fg)
 |}.
+Next Obligation. done. Qed.
 Next Obligation.
-  by intros V F A1 A2 B1 B2 n f g Hfg; apply stypeC_map_ne, cFunctor_ne.
+  by intros V F A1 ? A2 ? B1 ? B2 ? n f g Hfg;
+  apply stypeC_map_ne, cFunctor_ne.
 Qed.
 Next Obligation.
-  intros V F A B x. rewrite /= -{2}(stype_fmap_id x).
+  intros V F A ? B ? x. rewrite /= -{2}(stype_fmap_id x).
   apply stype_map_ext=>y. apply cFunctor_id.
 Qed.
 Next Obligation.
-  intros V F A1 A2 A3 B1 B2 B3 f g f' g' x. rewrite /= -stype_fmap_compose.
+  intros V F A1 ? A2 ? A3 ? B1 ? B2 ? B3 ? f g f' g' x.
+  rewrite /= -stype_fmap_compose.
   apply stype_map_ext=>y; apply cFunctor_compose.
 Qed.
 
 Instance stypeCF_contractive {V} F :
   cFunctorContractive F → cFunctorContractive (@stypeCF V F).
 Proof.
-  by intros ? A1 A2 B1 B2 n f g Hfg; apply stypeC_map_ne, cFunctor_contractive.
+  by intros ? A1 ? A2 ? B1 ? B2 ? n f g Hfg;
+  apply stypeC_map_ne, cFunctor_contractive.
 Qed.
 
 Class IsDualAction (a1 a2 : action) :=
@@ -253,7 +303,7 @@ Section DualStype.
   Proof. by rewrite /IsDualStype. Qed.
 
   Global Instance is_dual_end : IsDualStype (TEnd : stype V A) TEnd.
-  Proof. constructor. Qed.
+  Proof. by rewrite /IsDualStype -(stype_force_eq (dual_stype _)). Qed.
 
   Global Instance is_dual_tsr a1 a2 P (st1 st2 : V → stype V A) :
     IsDualAction a1 a2 →
@@ -261,7 +311,7 @@ Section DualStype.
     IsDualStype (TSR a1 P st1) (TSR a2 P st2).
   Proof.
     rewrite /IsDualAction /IsDualStype. intros <- Hst.
-    by constructor=> x.
+    rewrite /IsDualStype -(stype_force_eq (dual_stype _)) /=.
+    by constructor=> v.
   Qed.
-
 End DualStype.
